# Chapter 3.3 - Circular Orbits ($e = 0$)

For circular orbits, $e = 0$ and the right hand side of the integral becomes:

$$\frac{\mu}{h^3}t = \int_0^{\theta}d\theta = \theta$$

For a circle, the orbit formula is:

$$r = \frac{h^2}{\mu}$$

such that:

```{margin}
**Note:** There's a typo in the equation for $t$ in the book, it has a $\sqrt{\mu^2}$ in the denominator.
```

$$t = \frac{r^{3/2}}{\sqrt{\mu}}\theta$$

Since the period of the circular orbit is

$$T = \frac{2\pi}{\sqrt{\mu}}r^{3/2}$$

the time since periapsis can be rewritten as:

$$t = \frac{\theta}{2\pi}T$$

or, rearranging:

$$\theta = \frac{2\pi}{T}t$$

Note that the true anomaly is directly proportional to the elapsed time since periapsis. This is a consequence of the fact that circular orbits have constant angular velocity.

Moreover, since circles are symmetrical, the choice of apse line, and therefore the location of periapsis, is totally arbitrary, and we can pick any location on the circle to be periapsis and define $t = 0$.
